wrote implementation starting point

impl/src/Self.hs
@@ -1,4 +1,5 @@
 {-# LANGUAGE LambdaCase #-}
+{-# LANGUAGE DeriveFunctor #-}
 {-# LANGUAGE MultiWayIf #-}
 module Self where
 
@@ -29,68 +30,142 @@ data Com
   | Loop Com
   deriving (Show, Read, Eq, Ord)
 
-data Error = Error
+data St
+  = SID Int
+  | SPair St St
+  deriving (Show, Read, Eq, Ord)
 
-type M a = StateT Int (Either Error) a
+type ID = Int
 
-fresh :: M Prop
-fresh = undefined
+data Tree a
+  = Leaf a
+  | Branch (Tree a) (Tree a)
+  deriving (Functor, Show, Read, Eq, Ord)
 
-pairwise :: Prop -> Prop -> Prop
-pairwise = undefined
+type Shape = Tree ID
 
-clause :: Prop -> Prop -> M ()
+type Vocab = Tree [Var]
+
+type Rename = Tree (Var -> Var)
+
+data Assertion = Assertion
+  { shape :: Shape
+  , fact :: Rename -> Prop
+  }
+
+commute :: Assertion -> Assertion
+commute (Assertion (Branch s0 s1) phi) =
+  Assertion (Branch s1 s0)
+            (\case
+                Branch r0 r1 -> phi (Branch r1 r0)
+                _ -> undefined)
+commute _ = undefined
+
+associate :: Assertion -> Assertion
+associate (Assertion (Branch s0 (Branch s1 s2)) phi) =
+  Assertion (Branch (Branch s0 s1) s2)
+            (\case
+                Branch r0 (Branch r1 r2) -> phi (Branch r0 (Branch r1 r2))
+                _ -> undefined)
+associate _ = undefined
+
+mkAnd :: Assertion -> Assertion -> Assertion
+mkAnd (Assertion s0 phi0) (Assertion _ phi1) =
+  Assertion s0 (\r -> phi0 r `And` phi1 r)
+
+pairwise :: Assertion -> Assertion -> Assertion
+pairwise (Assertion s0 phi0) (Assertion s1 phi1) =
+  Assertion (Branch s0 s1)
+            (\case
+              Branch r0 r1 -> And (phi0 r0) (phi1 r1)
+              _ -> undefined)
+
+type M a = State Int a
+
+freshRel :: M Assertion
+freshRel = undefined
+
+clause :: Assertion -> Assertion -> M ()
 clause = undefined
+
+mkAssertion :: Prop -> Assertion
+mkAssertion = undefined
+
+andE :: Assertion -> Prop -> Assertion
+andE a p = mkAnd a (mkAssertion p)
 
 subst = undefined
 
 loopless :: Com -> Bool
-loopless = undefined
+loopless = \case
+  Loop{} -> False
+  Sum c0 c1 -> loopless c0 && loopless c1
+  Prod c0 c1 -> loopless c0 && loopless c1
+  Seq c0 c1 -> loopless c0 && loopless c1
+  Assert{} -> True
+  Assign{} -> True
+  Skip -> True
 
-allLoops :: Com -> Bool
-allLoops = undefined
+mergeLoops :: Com -> Com
+mergeLoops = \case
+  Prod c0 c1 ->
+    let c0' = mergeLoops c0
+        c1' = mergeLoops c1
+    in case (c0', c1') of
+         (Loop c0, Loop c1) -> Loop (Prod (Sum c0 Skip) (Sum c1 Skip))
+         _ -> Prod c0' c1'
+  c -> c
 
-dispatch :: Com -> Prop -> M Prop
+dispatch :: Com -> Assertion -> M Assertion
 dispatch c q =
   case c of
     Assign x e ->
       pure (subst x e q)
     Assert e -> do
-      p <- fresh
-      clause (And p e) q
+      p <- freshRel
+      clause (andE p e) q
       pure p
     Skip -> pure q
-    Seq c0 c1 -> do
-      r <- fresh
-      p <- dispatch c0 r
-      pr <- dispatch (Prod c0 c1) (pairwise r q)
-      clause (pairwise p r) pr
-      pure p
+    Seq c0 c1 ->
+      if loopless c0 || loopless c1
+      then do
+        r <- dispatch c1 q
+        dispatch c0 r
+      else do
+        r <- freshRel
+        p <- dispatch c0 r
+        pr <- dispatch (Prod c0 c1) (pairwise r q)
+        clause (pairwise p r) pr
+        pure p
     Sum c0 c1 -> do
-      p <- fresh
+      p <- freshRel
       p0 <- dispatch c0 q
       p1 <- dispatch c1 q
       clause p p0
       clause p p1
       pure p
-    Prod c0 c1 -> do
-      if | loopless c0 || loopless c1 -> do
-           q0 <- fresh
-           q1 <- fresh
-           p0 <- dispatch c0 q0
-           p1 <- dispatch c1 q1
-           p <- fresh
-           clause p p0 -- TODO
-           clause p p1 -- TODO
-           clause (pairwise q0 q1) q -- TODO
-           pure p
-         -- | allLoops c0 && allLoops c1 -> do
-         --   p <- fresh
-         --   let c0
-         | otherwise ->
-           case (c0, c1) of
-             (Sum c0' c0'', _) -> dispatch (Sum (Prod c0' c1) (Prod c0'' c1)) q
-             (_, Sum c1' c1'') -> dispatch (Sum (Prod c0 c1') (Prod c0 c1'')) q
-             (Seq c0' c0'', Seq c1' c1'') -> dispatch (Seq (Prod c0' c1') (Prod c0'' c1'')) q
-    Loop c0 -> do
-
+    Loop c -> do
+      p <- freshRel
+      r <- dispatch c p
+      clause r p
+      clause p q
+      pure p
+    Prod c0 c1 ->
+      if loopless c0 || loopless c1
+      then do
+        p <- freshRel
+        q0 <- freshRel
+        q1 <- freshRel
+        p0 <- dispatch c0 q0
+        p1 <- dispatch c1 q1
+        -- TODO these clauses are not precise.
+        clause (mkAnd q0 q1) q
+        clause p p0
+        clause p p1
+        pure p
+      else
+        case mergeLoops c1 of
+          Sum c1' c1'' -> dispatch (Sum (Prod c0 c1') (Prod c0 c1'')) q
+          Prod c1' c1'' -> dispatch (Prod (Prod c0 c1') c1'') (associate q)
+          Loop c1' -> dispatch (Prod (Loop c1') c0) (commute q)
+          _ -> error ("Some impossible state has been reached: `" ++ show c ++ "`.")
